Progress

coq-osiris/theories/program_logic/pure/spec_rules.v
@@ -85,8 +85,7 @@ Proof. intros; simpl_eval; by eapply pure_ret; eauto. Qed.
   In the second subgoal, we prove [e2] while abstracting over [e]. *)
 
 Local Lemma pure_eval_letrec_unary `{Encode X, Encode Y}
-  (P : _ -> microvx -> Prop) η f (x : var) e
-  e2 (φ : Y -> Prop) ζ
+  (P : _ -> microvx -> Prop) η f (x : var) e1 e2 (φ : Y -> Prop) ζ
   (* Show that the relation on which arguments are decreasing is well-founded. *)
   {WF_x : WellFounded X} :
   (* Show the specification [P] holds over a call to any argument
@@ -94,11 +93,11 @@ Local Lemma pure_eval_letrec_unary `{Encode X, Encode Y}
     argument [yval] smaller than [arg]. *)
   (∀ c (arg : X),
       Spec_Unary c (λ yval m, wf_relation (WF := WF_x) yval arg -> P yval m) ->
-      P arg (eval ((x, #arg) :: (f, c) :: η) e)) ->
+      P arg (eval ((x, #arg) :: (f, c) :: η) e1)) ->
   (* Continue with [f] bound to [c], and [c] specified by [P]. *)
   (∀ c, Spec_Unary c P -> pure (eval ((f, c) :: η) e2) φ ζ) ->
   (* When facing an expression of the form [let rec f x = e in e2]. *)
-  pure (eval η (ELetRec [RecBinding f (AnonFun x e)] e2)) φ ζ.
+  pure (eval η (ELetRec [RecBinding f (AnonFun x e1)] e2)) φ ζ.
 Proof.
   intros Hmkspec_unary He2. simpl_eval. eapply He2.
   unfold Spec_Unary. intros v.
@@ -141,26 +140,41 @@ Definition closure (f : val) : option (env * anonfun) :=
   | _ => None
   end.
 
-Equations Spec (A : types) (η : env) (f : anonfun) (P : A -#> microvx -> Prop) : Prop :=
+Equations aSpec (A : types) (η : env) (f : anonfun) (P : A -#> microvx -> Prop) : Prop :=
 | Tbase X, η, f, P :=
     ∀ (x : X), P x (acall η f #x)
 | Tcons X TT, η, f, P :=
     ∀ (x : X),
-      pure_wp (acall η f #x)
+      pure (acall η f #x)
         (λ c, match closure c with
                 | None => False
-                | Some (η, f) => Spec TT η f (P x) end) ⊥.
+                | Some (η, f) => aSpec TT η f (P x) end) ⊥.
 
 (* [Spec] lifted to propositions over values. *)
 
-Definition Spec_val (A : types) (c : val) (P : A -#> microvx -> Prop) :=
+Definition aSpec_val (A : types) (c : val) (P : A -#> microvx -> Prop) :=
   match closure c with
     | None => False
-    | Some (η, f) => Spec A η f P
+    | Some (η, f) => aSpec A η f P
   end.
 
-Arguments Spec {A} η f P.
-Arguments Spec_val {A} c P.
+Arguments aSpec {A} η f P.
+Arguments aSpec_val {A} c P.
+
+(* Spec η (AnonFun x e) P <-> *)
+(* forall v, pure (eval ((x, v) :: η) e) (Spec_val P *)
+(*   eval ((x, v) :: η) e. *)
+
+(* -------------------------------------------------------------------------- *)
+
+
+Equations Spec (A : types) (ρ : val) (P : A -#> microvx -> Prop) : Prop :=
+| Tbase X, ρ, P :=
+    ∀ (x : X), P x (call ρ #x)
+| Tcons X TT, ρ, P :=
+    ∀ (x : X), pure_wp (call ρ #x) (λ c, Spec TT c (P x)) ⊥.
+
+Arguments Spec {A} ρ P.
 
 (* -------------------------------------------------------------------------- *)
 
@@ -168,22 +182,44 @@ Arguments Spec_val {A} c P.
 
 (* [Spec_mono] states that [Spec] is monotonic over specifications. *)
 
-Lemma Spec_mono {A : types} (P P' : A -#> microvx -> Prop) η f :
-  Spec η f P ->
+Lemma Spec_mono {A : types} (P P' : A -#> microvx -> Prop) c :
+  Spec c P ->
   (∀# args, ∀ m, P args m -> P' args m) ->
-  Spec η f P'.
+  Spec c P'.
 Proof.
-  revert η f.
-  induction A as [ | X HX arg_τ IH ]; intros η f HP Hmono.
+  revert c.
+  induction A as [ | X HX arg_τ IH ]; intros c HP Hmono.
   { simp Spec in HP |-*. intros x.
     apply Hmono. apply HP. }
   simp Spec in HP |-*; intros x.
   eapply pure_wp_mono_ret; [ apply HP | ].
-  cbn ; intros c' HSpec'. destruct (closure c') eqn: Hn; eauto.
-  destruct p; subst.
+  intros c' HSpec'.
   apply IH with (P := P x); [ apply HSpec' | ].
   rewrite tforall_unroll in Hmono. apply Hmono.
 Qed.
+
+(* -------------------------------------------------------------------------- *)
+
+(** Basic properties about [Spec]. *)
+
+(* [Spec_mono] states that [Spec] is monotonic over specifications. *)
+
+(* Lemma aSpec_mono {A : types} (P P' : A -#> microvx -> Prop) η f : *)
+(*   aSpec η f P -> *)
+(*   (∀# args, ∀ m, P args m -> P' args m) -> *)
+(*   aSpec η f P'. *)
+(* Proof. *)
+(*   revert η f. *)
+(*   induction A as [ | X HX arg_τ IH ]; intros η f HP Hmono. *)
+(*   { simp aSpec in HP |-*. intros x. *)
+(*     apply Hmono. apply HP. } *)
+(*   simp aSpec in HP |-*; intros x. *)
+(*   eapply pure_wp_mono_ret; [ apply HP | ]. *)
+(*   cbn ; intros c' HSpec'. destruct (closure c') eqn: Hn; eauto. *)
+(*   destruct p; subst. *)
+(*   apply IH with (P := P x); [ apply HSpec' | ]. *)
+(*   rewrite tforall_unroll in Hmono. apply Hmono. *)
+(* Qed. *)
 
 (* -------------------------------------------------------------------------- *)
 
@@ -217,7 +253,7 @@ Qed.
 
 Local Lemma pure_anonfun_Spec (A : types) η x e (P : A -#> microvx -> Prop) :
   pure_anonfun η (EAnonFun (AnonFun x e)) P ->
-  @Spec A η (AnonFun x e) P.
+  @Spec A (VClo η (AnonFun x e)) P.
 Proof.
   revert dependent x; revert η; revert dependent A.
   (* We do induction on the depth of the number or arguments that the function takes.*)
@@ -245,7 +281,7 @@ Qed.
 
 Lemma pure_eval_anonfun (A : types) (P : A -#> microvx -> Prop) η (x : var) e ζ :
   pure_anonfun η (EAnonFun (AnonFun x e)) P ->
-  pure (eval η (EAnonFun (AnonFun x e))) (λ c, Spec_val c P) ζ.
+  pure (eval η (EAnonFun (AnonFun x e))) (λ c, Spec c P) ζ.
 Proof.
   intros HP.
   simpl_eval; apply pure_wp_ret.
@@ -255,956 +291,59 @@ Qed.
 
 (* -------------------------------------------------------------------------- *)
 
-(* [prove_Spec_rec] gives an induction principle for [Spec] by
-   well-foundedness over the argument type. *)
+From osiris Require Import program_logic.pure.toplevel_rules.
 
-Lemma prove_Spec_rec
-  {A : types}
-  (R : A -> A -> Prop) ρ
-  (P : A -#> microvx -> Prop) :
-  WellFounded R ->
-  (∀# (args : A),
-    (∀# sargs, R sargs args -> Spec ρ P sargs) ->
-    Spec ρ P args)->
-  Spec ρ P.
+Lemma pure_eval_letrec (A : types)
+  (R : A -> A -> Prop) (* LATER : State that this relation is well-founded *)
+  (P : A -#> microvx -> Prop)
+  (f : var) η e φ δ :
+  (forall vf (x' : A),
+    (forall x,
+      R x x' ->
+      Spec vf
+        (tbind (fun (x' : A) (m : microvx) => x' = x /\ P x' m))) ->
+     Spec (VCloRec ((f, vf) :: η) [RecBinding f e] f) P) ->
+  struct_items (η, δ) [ILetRec [RecBinding f e]] φ.
 Proof.
-  intros Hwf HP.
-  apply aSpec_Spec; eauto.
-  intros args.
+Admitted.
 
-  induction args as [args IHR] using (well_founded_induction Hwf); clear Hwf.
-
-  rewrite forallArgs_forall in HP. specialize (HP args).
-  apply HP.
-  apply forallArgs_forall; apply IHR.
-Qed.
-
-(* We would like to provide a [prove_Spec_rec]-like reasoning rule to
-   the user. We can then improve the user experience by stepping
-   through the nested calls that result from the unfolding of
-   [aSpec c P args].
-
-   This is done by [unfold_spec], which syntactically fetches the body
-   of the function [c]. *)
-
-Section unfold_spec_aux_def.
-
-  Context (og_arg_τ : arg_type).
-  Context (Pog : og_arg_τ -#> microvx -> Prop).
-  Context (c : val).
-
-  Equations unfold_spec_aux (arg_τ : arg_type)
-    (η : env) (e : expr)
-    (P : arg_τ -#> microvx -> Prop) (R : og_arg_τ -> arg_τ -> Prop)
-    : Prop :=
-  | Arg1 X, η, (EAnonFun (AnonFun arg e)), P, R :=
-      ∀ (x : X),
-        Spec c (arg_bind(λ sargs m,
-                    R sargs x ->
-                    Pog sargs m)) ->
-        P x (eval ((arg, #x) :: η) e)
-  | ArgS X arg_τ', η, (EAnonFun (AnonFun arg e)), P, R :=
-      ∀ (x : X),
-        let η := (arg, #x) :: η in
-        let P := P x in
-        let R := (λ (sargs : og_arg_τ) (args : arg_τ'),
-                   R sargs {| arg_head := x; arg_tail := args |})
-        in
-        unfold_spec_aux arg_τ' η e P R
-  | _, _, _, _, _ := False.
-
-End unfold_spec_aux_def.
-
-Strategy transparent [ unfold_spec_aux ].
-
-Definition unfold_spec (arg_τ : arg_type) η f x e
-  (R : arg_τ -> arg_τ -> Prop)
-  (P : arg_τ -#> microvx -> Prop) :=
-  (∀ c, unfold_spec_aux arg_τ P c arg_τ ((f, c) :: η) (EAnonFun (AnonFun x e)) P R).
-
-Arguments unfold_spec arg_τ /.
-Strategy transparent [ unfold_spec ].
-
-Lemma aSpec_equiv (arg_τ : arg_type) η f x e (P : arg_τ -#> _) args :
-  aSpec (VCloRec η [RecBinding f (AnonFun x e)] f) P args =
-  aSpec (VClo ((f, VCloRec η [RecBinding f (AnonFun x e)] f) :: η) (AnonFun x e)) P args.
-Proof with Spec_auto.
-  destruct arg_τ...
-  { cbv; simp aSpec_aux.
-    simpl; rewrite String.eqb_refl; simpl. reflexivity. }
-  cbn...
-  simpl; rewrite String.eqb_refl; simpl. reflexivity.
-Qed.
-
-Lemma Spec_equiv (arg_τ : arg_type) η f x e (P : arg_τ -#> _) :
-  Spec (VCloRec η [RecBinding f (AnonFun x e)] f) P =
-    Spec (VClo ((f, VCloRec η [RecBinding f (AnonFun x e)] f) :: η) (AnonFun x e)) P.
-Proof with Spec_auto.
-  destruct arg_τ.
-  { cbv; simp Spec.
-    simpl; rewrite String.eqb_refl; reflexivity. }
-  simp Spec; simpl; rewrite String.eqb_refl; reflexivity.
-Qed.
-
-Definition is_VCloRec v e :=
-  ∃ η f x, v = VCloRec η [ RecBinding f (AnonFun x e) ] f.
-
-Fixpoint is_lambda_of_depth e (arg_τ : arg_type) : Prop :=
-  match arg_τ with
-  | Arg1 _ =>
-      exists x ebody,
-      e = EAnonFun (AnonFun x ebody)
-  | ArgS _ arg_τ' =>
-      exists x e',
-      e = EAnonFun (AnonFun x e') ∧ is_lambda_of_depth e' arg_τ'
-  end.
-
-Definition is_VCloRec_of_depth v arg_τ :=
-  exists η f x e,
-    v = VCloRec η [ RecBinding f (AnonFun x e) ] f ∧
-      match arg_τ with
-      | Arg1 _ => True
-      | ArgS _ arg_τ' =>
-          is_lambda_of_depth e arg_τ'
-      end.
-
-Lemma guarded_Spec_equiv (arg_τ arg_τ_og : arg_type) c
-  (R : arg_τ_og -> arg_τ -> Prop) (P : arg_τ_og -#> microvx -> Prop) (args : arg_τ) :
-  is_VCloRec_of_depth c arg_τ_og ->
-  Spec c (arg_bind(λ sargs m,
-              R sargs args ->
-              P sargs m)) <->
-  (∀# sargs, R sargs args -> aSpec c P sargs).
-Proof.
-  intros Hclo.
-  split; [ clear Hclo | ].
-  { revert c.
-    induction arg_τ_og as [ X H | X H arg_τ_og IH ]; intros c.
-    - unfold aSpec; simp Spec.
-      intros Hcall x HR.
-      rewrite args_app_bind.
-      simp aSpec_aux. apply Hcall. apply HR.
-    - intros HSpec.
-      rewrite spec_once; intros sx.
-      simp Spec in HSpec; specialize (HSpec sx).
-
-      apply forallArgs_forall; intros sargs HR.
-      unfold aSpec; rewrite args_app_bind; simp aSpec_aux.
-      eapply pure_wp_mono_ret; [ apply HSpec | ].
-      intros c' HSpec'.
-      specialize (IH (λ t1 t2, R (ArgCons sx t1) t2)).
-      specialize (IH (P sx)).
-      specialize (IH c').
-      specialize (IH HSpec').
-      rewrite forallArgs_forall in IH; specialize (IH sargs HR).
-      unfold aSpec in IH; rewrite args_app_bind in IH.
-      apply IH. }
-
-  intros HaSpec.
-
-  destruct Hclo as (η & f & x & e & -> & He).
-  assert (∀# sargs, R sargs args -> aSpec (VClo ((f, (VCloRec η [ RecBinding f (AnonFun x e)] f)) :: η) (AnonFun x e)) P sargs) as HSpec.
-  { apply forallArgs_forall; intros sargs HR.
-    rewrite forallArgs_forall in HaSpec; specialize (HaSpec sargs HR).
-    rewrite <- aSpec_equiv. apply HaSpec. }
-  clear HaSpec.
-  rewrite Spec_equiv.
-
-  generalize dependent ((f, VCloRec η [RecBinding f (AnonFun x e)] f) :: η).
-  revert dependent e.
-  revert x.
-  induction arg_τ_og as [ X H | X H arg_τ_og IH ]; intros x e He η0 HSpec.
-  { simp Spec; intros vx HR.
-    specialize (HSpec vx HR).
-    unfold aSpec in HSpec; rewrite args_app_bind in HSpec.
-    apply HSpec. }
-
-  simp Spec; intros sx. simpl.
-
-  destruct arg_τ_og.
-  { inversion He as (y & e' & ->).
-    simpl_eval. apply pure_wp_ret.
-    simp Spec; intros vy HR.
-    specialize (HSpec sx vy HR). simpl in HSpec.
-    unfold aSpec in HSpec.
-    cbv in HSpec. simp aSpec_aux in HSpec.
-    simpl in HSpec.
-    unfold eval in HSpec; rewrite seal_eq in HSpec; simpl in HSpec.
-    apply invert_pure_wp_ret in HSpec.
-    apply HSpec. }
-
-  inversion He as (y & e' & -> & He').
-  simpl_eval. apply pure_wp_ret.
-
-  specialize (IH (λ t1 t2, R (ArgCons sx t1) t2)).
-  specialize (IH (P sx)).
-  specialize (IH y e' He').
-  specialize (IH ((x, #sx) :: η0)).
-  apply IH.
-
-  rewrite spec_once in HSpec; specialize (HSpec sx).
-  apply forallArgs_forall; intros sargs HR.
-  rewrite forallArgs_forall in HSpec; specialize (HSpec sargs HR).
-  unfold aSpec in HSpec. rewrite args_app_bind in HSpec.
-  simp aSpec_aux in HSpec.
-  simpl in HSpec.
-  unfold eval in HSpec; rewrite seal_eq in HSpec; simpl in HSpec.
-  apply invert_pure_wp_ret in HSpec.
-  unfold aSpec; rewrite args_app_bind.
-  apply HSpec.
-Qed.
-
-Lemma invert_unfold_spec (arg_τ : arg_type) (args : arg_τ) η f x e R P :
-  unfold_spec arg_τ η f x e R P ->
-  is_VCloRec_of_depth (VCloRec η [RecBinding f (AnonFun x e)] f) arg_τ.
-Proof.
-  intros Huspec.
-  specialize (Huspec (VCloRec η [RecBinding f (AnonFun x e)] f)).
-  remember P as Pog in Huspec at 1; clear HeqPog.
-  remember arg_τ as TTog in R at 1, Pog, Huspec at 1; clear HeqTTog.
-
-  eexists _, _, _, _; split; [ reflexivity | ].
-  destruct arg_τ as [ | X HX arg_τ ]; [ done | ].
-  destruct args as [vx args]. revert Huspec.
-  generalize ((f, VCloRec η [RecBinding f (AnonFun x e)] f) :: η); intros η0.
-  generalize (VCloRec η [RecBinding f (AnonFun x e)] f) as v; intros v Huspec.
-
-  revert dependent e. revert dependent X. revert x η0.
-  induction arg_τ as [ Y HY | Y HY arg_τ' IH ]; intros x η0 X HX vx R P e Huspec.
-  { destruct e; try (specialize (Huspec vx); contradiction).
-    destruct a as [y e'].
-    eexists _, _; reflexivity. }
-
-  destruct e; try (specialize (Huspec vx); contradiction); destruct a as [y e'].
-  destruct args as [vy args].
-  specialize (IH args y ((x, #vx) :: η0) Y HY vy).
-  specialize (IH (λ t1 t2, R t1 (ArgCons vx t2)) (P vx)).
-  specialize (IH e').
-  eexists _, _; split; [ reflexivity | ].
-  apply IH.
-  simpl in Huspec. specialize (Huspec vx).
-  intros vyy.
-  simpl. specialize (Huspec vyy).
-  apply Huspec.
-Qed.
-
-Lemma by_unfold_spec (arg_τ : arg_type) η f x e R P :
-  let c := VCloRec η [RecBinding f (AnonFun x e)] f in
-  @unfold_spec arg_τ η f x e R P ->
-  (∀# args,
-    (∀# sargs, R sargs args -> aSpec c P sargs) ->
-    aSpec c P args).
-Proof with Spec_auto.
-  unfold unfold_spec; intros HP.
-  apply forallArgs_forall; intros args IHargs.
-  pose proof (invert_unfold_spec arg_τ args η f x e R P HP) as Hclo.
-  specialize (HP (VCloRec η [RecBinding f (AnonFun x e)] f)).
-
-  (* Generalize all instances of [(f, c) :: η]. *)
-  rewrite aSpec_equiv.
-  revert HP.
-  generalize ((f, VCloRec η [RecBinding f (AnonFun x e)] f) :: η); intros η0.
-  (* Generalize the [VCloRec] used in the recursive call. *)
-  revert IHargs Hclo.
-  generalize (VCloRec η [RecBinding f (AnonFun x e)] f); intros v.
-
-  (* Generalize (TeleS X TT) where it doesn't participate in the
-     recursion. This is exactly where [TTog] appears in the definition
-     of [Spec_AnonFun_rec_aux]. *)
-  intros IHargs Hclo HP.
-
-  remember P as Pog in HP at 1, IHargs; clear HeqPog.
-  remember arg_τ as TTog in R at 1, Pog, HP at 1, IHargs, Hclo; clear HeqTTog.
-
-  (* Generalize the statement for the induction. Notably, generalize
-     over the head type of the telescope. *)
-  revert x e η0 HP Hclo.
-  induction arg_τ as [ X HX | X HX arg_τ IH]; intros x e η0 Hbp Hclo.
-
-  (* Base case: the telescope is empty. *)
-  { cbv... apply Hbp.
-    apply <- (guarded_Spec_equiv (tele[X]) TTog _ R Pog args Hclo).
-
-    apply IHargs. }
-
-  (* Induction step: the telescope has some head type [Y]. *)
-  destruct args as [vx args].
-  simpl in Hbp. specialize (Hbp vx).
-
-  (* We know that [e = EAnonFun (AnonFun y e')] by inversion on Hbp. *)
-  destruct e;
-    ((destruct arg_τ; contradiction)
-     || destruct a as [y e']).
-
-  (* Specialize the induction hypothesis before destructing args. *)
-  specialize (IH (λ ttog tt,
-                  R ttog {| arg_head := vx; arg_tail := tt |})).
-  specialize (IH (P vx) args).
-  specialize (IH IHargs).
-  specialize (IH y e' ((x, #vx) :: η0)).
-  (* We now step forward by evaluating [pure (eval .. (EAnonFun y e')) (λ c', ..)]. *)
-  simpl... simp aSpec_aux.
-  simpl; simpl_eval; simpl.
-  apply pure_wp_ret.
-
-  apply IH. apply Hbp.
-  apply Hclo.
-Qed.
-
-(* -------------------------------------------------------------------------- *)
-
-(* [pure_eval_letrec] is the user-facing lemma for reasoning about an
-   n-ary letrec. Its statement makes use of [unfold_spec] to generate
-   an appropriate lemma for every arity. *)
-
-(** For example, if we have [arg_τ := tele[ list Z; Nat ] ],
-    [pure_eval_letrec] becomes equal to
-
-    Lemma pure_eval_letrec (P : list Z -> Nat -> microvx -> Prop)
-    (R : (list Z * Nat) -> (list Z * Nat) -> Prop)
-    η f x e e2 φ ζ :
-    wf R ->
-    (∀ c (l : list Z) (n : Nat),
-       (∀ (l' : list Z) (n' : Nat), R (l', n') (l, n) -> aSpec c P l' n') ->
-       P l n (eval ((y, n) :: (x, l) :: (f, c) :: η) e)) ->
-    (∀ c, Spec c P -> pure (eval ((f, c) :: η) e2) φ ζ) ->
-    pure (eval η (ELetRec [RecBinding f (AnonFun x (EAnonFun (AnonFun y e)))] e2)) φ ζ.
-
-*)
-
-Lemma pure_eval_letrec `{Encode X} (arg_τ : arg_type) `{Inhabited arg_τ}
-  (P : arg_τ -#> microvx -> Prop)
-  (R : to_product_type arg_τ -> to_product_type arg_τ -> Prop) η f (x : var) e
-  e2 (φ : X -> Prop) ζ :
+Local Lemma pure_eval_letrec' `{Encode X, Encode Y}
+  (P : call_spec') (R : X -> X -> Prop) η f (x : var) e
+  e2 (φ : Y -> Prop) ζ :
   (* Show that the relation on which arguments are decreasing is well-founded. *)
   wf R ->
-  (* Show the specification [P] holds over a call to any arguments,
-     under the assumption that [P] holds to a call over any
-     smaller arguments. *)
-  unfold_spec arg_τ η f x e
-    (λ arg1 arg2, R (to_tuple arg1) (to_tuple arg2)) P ->
+  (* Show the specification [P] holds over a call to any argument
+    [arg], under the assumption that [P] holds to a call over any
+    argument [yval] smaller than [arg]. *)
+  (∀ c (arg : X),
+      Spec' c (λ yval m, R yval arg -> P yval m) ->
+      P arg (eval ((x, #arg) :: (f, c) :: η) e)) ->
   (* Continue with [f] bound to [c], and [c] specified by [P]. *)
-  (∀ c, Spec c P -> pure (eval ((f, c) :: η) e2) φ ζ) ->
+  (∀ c, Spec' c P -> pure (eval ((f, c) :: η) e2) φ ζ) ->
   (* When facing an expression of the form [let rec f x = e in e2]. *)
   pure (eval η (ELetRec [RecBinding f (AnonFun x e)] e2)) φ ζ.
 Proof.
-  intros Hwf Hmkspec He2. simpl_eval. eapply He2.
-  eapply prove_Spec_rec; eauto.
-  apply by_unfold_spec.
-  apply Hmkspec.
-Qed.
 
 
-(* [pure_eval_anonfun_nonrec] is to be used when a letrec expression
-   defines a non-recursive function.  *)
-
-Lemma pure_eval_letrec_nonrec `{Encode X} (arg_τ : arg_type)
-  (P : arg_τ -#> microvx -> Prop) η f x e e2 (φ : X -> Prop) ζ :
-  let v := VCloRec η [RecBinding f (AnonFun x e)] f in
-  (* Show the specification [P] holds over a call to any argument. *)
-  (Spec_AnonFun arg_τ ((f, v) :: η) (EAnonFun (AnonFun x e)) P) ->
-  (* Continue with [f] bound to [c], and [c] specified by [P]. *)
-  (∀ c, Spec c P -> pure (eval ((f, c) :: η) e2) φ ζ) ->
-  (* When facing an expression of the form [let rec f x = e in e2]. *)
-  pure (eval η (ELetRec [RecBinding f (AnonFun x e)] e2)) φ ζ.
-Proof.
-  intros v Hmkspec He2. simpl_eval. eapply He2.
-  pose proof (prove_Spec _ _ _ _ _ Hmkspec) as HSpec.
-  destruct arg_τ;
-    simp Spec;
-    simpl in *; rewrite String.eqb_refl; apply HSpec.
-Qed.
-
-
-(* [pure_call_spec'] illustrates how we may want to use a [Spec c P]
-   specification. *)
-
-Local Lemma pure_call_spec' `{Encode X, Encode Y} (P : X -> microvx -> Prop) c v (φ : Y -> Prop) ζ :
-  Spec' c P ->
-  (∀ m, P v m -> pure m φ ζ) ->
-  pure (eval.call c #v) φ ζ.
-Proof.
-  intros HSpec Hmon. eapply pure_call_equiv.
-  apply Hmon. apply HSpec.
-Qed.
-
-(* [pure_EApp_partial] is a lemma for partial application. *)
-
-Lemma pure_EApp_partial `{Encode X} (arg_τ: arg_type) η e e1 ζ
-  (φ1 : X -> Prop) (P : ArgS X arg_τ -#> microvx -> Prop) :
-  pure (eval η e) (λ c, Spec c P) ζ ->
-  pure (eval η e1) φ1 ζ ->
-  pure (eval η (EApp e e1)) (λ c, ∃ v1, φ1 v1 ∧ Spec c (P v1)) ζ.
-Proof.
-  intros.
-  eapply pure_eval_app; eauto.
-  intros c v1 Hc Hv1.
-  apply pure_call_equiv. simpl in Hc.
-  eapply pure_wp_mono. simp Spec in Hc.
-  - intros c' Hc'. unfold returns; eexists; split; [ reflexivity | ].
-    eauto.
-  - intros ? [].
-Qed.
-
-Lemma pure_EApp_partial_alt `{Encode X} (arg_τ : arg_type) η e e1 ζ
-  (φ1 : X -> Prop) (P : ArgS X arg_τ -#> microvx -> Prop) :
-  pure (eval η e) (λ c, Spec c P) ζ ->
-  pure (eval η e1) φ1 ζ ->
-  pure (eval η (EApp e e1))
-    (λ c,
-      Spec c (arg_bind (λ (tt : arg_τ) m,
-                  ∃ (x : X),
-                      arg_app P
-                      {|
-                        arg_head := x ;
-                        arg_tail := tt
-                      |} m ∧
-                      φ1 x))
-    )
-    ζ.
-Proof.
-  intros.
-  eapply pure_eval_app; eauto.
-  intros c v1 Hc Hv1.
-  apply pure_call_equiv. simpl in Hc.
-  eapply pure_wp_mono. simp Spec in Hc.
-  - intros c' Hc'. unfold returns; eexists; split; [ reflexivity | ].
-    eapply Spec_mono; [ apply Hc' | ].
-    apply forallArgs_forall; intros args m HP.
-    rewrite args_app_bind.
-    exists v1. split; [ apply HP | apply Hv1 ].
-  - intros ? [].
-Qed.
-
-(* The following lemmas illustrate that we can reach our desired
-   reasoning rule using chained applications of [pure_EApp_partial] or
-   [pure_EApp_partial_alt]. *)
-
-(* Although we still are missing a single lemma for n-ary applications,
-   this demonstrates that a user could repeatedly use the partial
-   application lemmas to prove an n-ary application. *)
-
-Local Lemma pure_EApp_prop2 `{Encode A, Encode B, Encode C} η e e1 e2 (Ψ : C -> Prop) ζ
-  (φ1 : A -> Prop) (φ2 : B -> Prop) (P : tele[A; B] -#> microvx -> Prop) :
-  pure (eval η e) (λ c, Spec c P) ζ ->
-  pure (eval η e1) φ1 ζ ->
-  pure (eval η e2) φ2 ζ ->
-  (∀ v1 v2, φ1 v1 -> φ2 v2 -> ∀ m, P v1 v2 m -> pure m Ψ ζ) ->
-  pure (eval η (EApp (EApp e e1) e2)) Ψ ζ.
-Proof.
-  intros He He1 He2 Hmono.
-  eapply pure_eval_app; eauto.
-  eapply pure_EApp_partial; eauto. simpl.
-  intros c v2 (v1 & HP & Hv1) Hv2.
-  apply pure_call_equiv.
-  eapply Hmono; eauto. simp Spec in Hv1.
-Qed.
-
-Local Lemma pure_EApp_prop3 `{Encode A, Encode B, Encode C, Encode D} η e e1 e2 e3 (Ψ : D -> Prop) ζ
-  (φ1 : A -> Prop) (φ2 : B -> Prop) (φ3 : C -> Prop) (P : tele[A; B; C] -#> microvx -> Prop) :
-  pure (eval η e) (λ c, Spec c P) ζ ->
-  pure (eval η e1) φ1 ζ ->
-  pure (eval η e2) φ2 ζ ->
-  pure (eval η e3) φ3 ζ ->
-  (∀ v1 v2 v3, φ1 v1 -> φ2 v2 -> φ3 v3 -> ∀ m, P v1 v2 v3 m -> pure m Ψ ζ) ->
-  pure (eval η (EApp (EApp (EApp e e1) e2) e3)) Ψ ζ.
-Proof.
-  intros He He1 He2 He3 Hmono.
-  eapply pure_eval_app; eauto.
-  (* Here either could also use [pure_EApp_partial]. *)
-  eapply pure_EApp_partial_alt; eauto.
-  eapply pure_EApp_partial_alt; eauto.
-  intros c v3 HSpec Hv3; simpl in HSpec.
-  destruct (HSpec v3) as (v2 & (v1 & HP & Hv2) & HH).
-  apply pure_call_equiv.
-  eapply Hmono; eauto.
-Qed.
-
-(* -------------------------------------------------------------------------- *)
-
-(* We provide a gallina function [pure_EApp_prop], which computes a
-   proposition from an argument type. This proposition generalises
-   [pure_EApp_prop2] to n-ary applications. *)
-
-Fixpoint app_exprs e (es : list expr) :=
-  match es with
-  | [] => e
-  | e' :: es =>
-      EApp (app_exprs e es) e'
-  end.
-
-Section pure_EApp_prop_aux_def.
-
-  Context (η : env) (ζ : exn -> Prop).
-  Context (expr_base : expr) (goal_hyp : expr -> Prop).
-
-  Equations pure_EApp_prop_aux (arg_τ : arg_type)
-    (es : list expr) (mon_acc : arg_τ -#> Prop -> Prop) : Prop :=
-  | Arg1 X, es, mon_acc :=
-      ∀ (e : expr) (φ : X -> Prop),
-        pure (eval η e) φ ζ ->
-        let Hmono := ∀ (x : X), mon_acc x (φ x) in
-        (* [nested_eapp] is the nested application from [expr_base] and [exprs]. *)
-        let nested_eapp := app_exprs expr_base (e :: es) in
-        (* we want to prove [goal_hyp], i.e. that evaluating the nested
-           application satisfies [Ψ]. *)
-        let goal_hyp := goal_hyp nested_eapp in
-        (* [all_hyps] is the list of all hypotheses that we will chain with [->] arrows. *)
-        Hmono -> goal_hyp
-  | ArgS X arg_τ', es, mon_acc :=
-      (* Quantify over the expression of a new argument and its postcondition. *)
-      ∀ (e : expr) (φ : X -> Prop),
-        pure (eval η e) φ ζ ->
-        (* Add [e] to our list of expressions. *)
-        let es' := e :: es in
-        (* Add the hypothesis that evaluating [e] produces a value
-            over which [φ] holds to our list of hypotheses. *)
-        let mon_acc :=
-          arg_bind (λ (tt : arg_τ') (B : Prop),
-              ∀ (x : X),
-                φ x ->
-                (arg_app mon_acc {| arg_head := x; arg_tail := tt |} B))
-        in
-        pure_EApp_prop_aux arg_τ' es' mon_acc.
-
-  Arguments pure_EApp_prop_aux !arg_τ /.
-  Transparent pure_EApp_prop_aux.
-
-End pure_EApp_prop_aux_def.
-
-Definition pure_EApp_prop (arg_τ : arg_type) (η : env) (e : expr) (Ψ : val -> Prop)
-  (ζ : exn -> Prop) (P : arg_τ -#> microvx -> Prop) : Prop :=
-  pure (eval η e) (λ c, Spec c P) ζ ->
-  pure_EApp_prop_aux η ζ e (λ e, pure (eval η e) Ψ ζ)
-    arg_τ
-    []
-    (arg_bind (λ (tt : arg_τ) (B : Prop),
-         B -> ∀ m, (arg_app P tt) m -> pure m Ψ ζ)).
-
-Arguments pure_EApp_prop !arg_τ /.
-Transparent pure_EApp_prop.
-
-(* We always want [pure_EApp_prop] to unfold, the user should only be
-   exposed to the generated lemma. *)
-
-Strategy transparent [ pure_EApp_prop pure_EApp_prop_aux ].
-
-(* The lemmas generated by [pure_EApp_prop] are monotonic in the
-   consequence hypothesis. *)
-
-Local Lemma pure_EApp_mono (arg_τ : arg_type) (η : env) ζ e fe es
-  (Hmon' Hmon : arg_τ -#> Prop -> Prop) :
-  pure_EApp_prop_aux η ζ e fe arg_τ es Hmon' ->
-  (∀ args P, Hmon args P -> Hmon' args P) ->
-  pure_EApp_prop_aux η ζ e fe arg_τ es Hmon.
-Proof.
-  revert es.
-  induction arg_τ as [ X HX | X HX TT IH ];
-    intros es HEApp' Hmono; simpl; intros ex φx Hex.
-  { intros Hx.
-    simp pure_EApp_prop_aux in HEApp'.
-    eapply HEApp'. apply Hex.
-    intros x; apply Hmono; apply Hx. }
-
-  eapply IH; [ apply HEApp' | ]. apply Hex.
-  intros args P; rewrite !args_app_bind.
-  intros Hx x Hφ.
-  apply Hmono. apply Hx. apply Hφ.
-Qed.
-
-Local Lemma pure_EApp_prop_induction_step (arg_τ : arg_type) (η : env) e
-  (ζ : exn -> Prop) f :
-  ∀ (Hmono : arg_τ -#> Prop -> Prop) (es : list expr) (ei : expr),
-    app_exprs (EApp e ei) es = app_exprs e (es ++ [ei]) ->
-    pure_EApp_prop_aux η ζ
-      (EApp e ei)
-      (λ e0, f e0) arg_τ
-      es
-      Hmono ->
-    pure_EApp_prop_aux η ζ
-      e
-      (λ e0, f e0) arg_τ
-      (es ++ [ei])
-      Hmono.
-Proof.
-  induction arg_τ as [ X HX | X HX TT IH ];
-    intros Hmono es ei HeqEApp Happlied.
-  { simpl in *; rewrite <- HeqEApp; apply Happlied. }
-
-  intros ex φx Hx; cbn zeta.
-  simp pure_EApp_prop_aux in Happlied.
-  specialize (IH (arg_bind (λ (tt : TT) (B : Prop),
-            ∀ x : X,
-              φx x →
-              arg_app
-                Hmono
-                {|
-                  arg_head := x ;
-                  arg_tail := tt
-                |} B))).
-  specialize (IH (ex :: es) ei).
-  apply IH; [ simpl; f_equal; apply HeqEApp | ].
-  apply Happlied. apply Hx.
-Qed.
-
-Lemma pure_EApp (arg_τ : arg_type) η e Ψ ζ (P : arg_τ -#> microvx -> Prop) :
-  pure_EApp_prop arg_τ η e Ψ ζ P.
-Proof.
-  (* Unfold [pure_EApp_prop]. *)
-  unfold pure_EApp_prop.
-
-  (* We proceed by induction on [arg_τ]. *)
-  revert e.
-  induction arg_τ as [ X HX | X HX arg_τ IH];
-    intros e HSpec ex φx Hx; cbn zeta.
-
-  { (* Base case. *)
-    intros Hmono; simpl in Hmono.
-    eapply pure_eval_app; eauto.
-    intros c x Hc Hφx. apply pure_call_equiv.
-    eapply Hmono; [ apply Hφx | ].
-    simpl in Hc; simp Spec in Hc; apply Hc. }
-
-  (* General case: our aim is to use [worse_pure_EApp_induction_step]. *)
-  change [ex] with ([] ++ [ex]).
-  apply pure_EApp_prop_induction_step; [ reflexivity | ].
-
-  (* Specialize the induction hypothesis with a
-     [P' : TeleS Y TT -#> microvx -> Prop] such that
-     [pure (eval η (EApp e ex)) (λ c, Spec c P')] and
-     [∀# args, ∀ B, P' args B -> (∀ x, φ x -> B -> ∀ m, (P x) args m -> pure m Ψ ζ)]. *)
-  specialize (IH (arg_bind (λ (tt : arg_τ) m,
-                      ∃ x,
-                        φx x ∧
-                          (arg_app
-                             P
-                             {|
-                               arg_head := x;
-                               arg_tail := tt |}
-                          ) m))).
-  specialize (IH (EApp e ex)).
-
-  (* Use the induction hypothesis. *)
-  eapply pure_EApp_mono; [ eapply IH | ].
-
-  { (* Subgoal: [ pure (eval η (EApp e ex)) (λ c, Spec c P') ζ ]. *)
-    eapply pure_eval_app; eauto.
-    intros c x Hc Hφx. eapply pure_call_equiv.
-    eapply pure_wp_mono. simpl in Hc; simp Spec in Hc; apply Hc.
-    - intros c' HSpec'; cbn beta in HSpec'.
-      unfold returns; eexists; split; [ reflexivity | ].
-      eapply Spec_mono; [ apply HSpec' | ].
-      apply forallArgs_forall; intros args m HP.
-      rewrite args_app_bind.
-      exists x; split; [ apply Hφx | apply HP ].
-    - intros ? []. }
-
-  (* Subgoal:
-     [ ∀# args, ∀ B,
-       P' args B ->
-       ∀ x, φx x -> B ->
-       ∀ m, (P x) arg m -> pure m Ψ ζ ]. *)
-  intros args B.
-  rewrite !args_app_bind. intros Hmon HB m (x & Hφx & HP).
-  specialize (Hmon x Hφx). rewrite args_app_bind in Hmon.
-  eapply Hmon; eauto.
-Defined.
-
-(* -------------------------------------------------------------------------- *)
-
-(* [pure_EApp_prop] generates a lemma that allows us to use our [Spec]
-   hypotheses. [pure_EApp_aSpec] is essentially the same, but for using
-   [aSpec] hypotheses. *)
-
-(* An example of the shape we want [pure_EApp_aSpec] lemmas to take: *)
-
-Local Lemma pure_EApp_aSpec1 `{Encode X, Encode Y} η e e2
-  (P : tele[X] -#> microvx -> Prop) (Ψ : Y -> Prop) ζ
-  :
-  ∀# (sargs : Arg1 X),
-  pure (eval η e) (λ c, aSpec c P sargs) ζ ->
-  pure (eval η e2) (singleton sargs) ζ ->
-  (∀ m, P sargs m -> pure m Ψ ζ) ->
-  pure (eval η (EApp e e2)) Ψ ζ.
-Proof.
-  apply forallArgs_forall; intros args He He2 Hmono.
-  eapply pure_eval_app; eauto.
-  intros c x Hc ->.
-  apply pure_call_equiv.
-  apply Hmono. apply Hc.
-Qed.
-
-Section pure_EApp_aSpec_def.
-
-  Context (η : env) (ζ : exn -> Prop).
-  Context (expr_base : expr) (goal_hyp : expr -> Prop).
-
-  Equations pure_EApp_aSpec (arg_τ : arg_type) (args : arg_τ) (exprs : list expr) : Prop :=
-  | Arg1 X, x, exprs :=
-      ∀ (e : expr),
-        pure (eval η e) (singleton x) ζ ->
-        let nested_eapp := app_exprs expr_base (e :: exprs) in
-        goal_hyp nested_eapp
-  | ArgS X arg_τ', {| arg_head := x; arg_tail := args' |}, exprs :=
-       ∀ (e : expr),
-         pure (eval η e) (singleton x) ζ ->
-         pure_EApp_aSpec arg_τ' args' (e :: exprs).
-
-End pure_EApp_aSpec_def.
-
-Strategy transparent [ pure_EApp_aSpec ].
-
-Lemma pure_EApp_aSpec_induction_step (arg_τ : arg_type) η e ζ f :
-  ∀ args (es : list expr) (ei : expr),
-    app_exprs (EApp e ei) es = app_exprs e (es ++ [ei]) ->
-    pure_EApp_aSpec η ζ
-      (EApp e ei)
-      (λ e  : expr, f e)
-      arg_τ
-      args
-      es  ->
-    @pure_EApp_aSpec η ζ
-      e
-      (λ e  : expr, f e)
-      arg_τ
-      args
-      (es ++ [ei]).
-Proof with Spec_auto.
-  induction arg_τ as [ X HX | X HX TT IH ]; intros args es ei Heqapp Heapp...
-
-  { simpl in *. rewrite <- Heqapp. apply Heapp. }
-
-  intros ex Hex.
-
-  specialize (IH arg_tail (ex :: es) ei).
-
-  apply IH. { simpl. f_equal. apply Heqapp. }
-  apply Heapp. apply Hex.
-Qed.
-
-(* The lemmas generated by [pure_EApp_aSpec] are monotonic in the goal
-   hypothesis. *)
-
-Local Lemma pure_EApp_aSpec_mono (arg_τ : arg_type) η e ζ args es
-  (f f' : expr -> Prop) :
-  pure_EApp_aSpec η ζ
-    e
-    (λ e0  : expr, f' e0)
-    arg_τ
-    args
-    es  ->
-  (∀ e, f' e -> f e) ->
-  @pure_EApp_aSpec η ζ
-    e
-    (λ e0  : expr, f e0)
-    arg_τ
-    args
-    es.
-Proof with Spec_auto.
-  intros HEApp Hmono.
-  revert HEApp. revert es.
-  induction arg_τ; intros es...
-Qed.
-
-Lemma pure_EApp' `{Encode Y} (arg_τ : arg_type) η e (Ψ : Y -> Prop) ζ
-  (P : arg_τ -#> microvx -> Prop) :
-  ∀# (args : arg_τ),
-    @pure_EApp_aSpec η ζ
-      e
-      (λ e0, pure (eval η e) (λ c, aSpec c P args) ζ ->
-             (∀ m, P args m -> pure m Ψ ζ) ->
-             pure (eval η e0) Ψ ζ)
-      arg_τ
-      args
-      [].
-Proof with Spec_auto.
-  apply forallArgs_forall; intros args.
-  revert e.
-  induction arg_τ as [ X HX | X HX TT IH]; intros e...
-  { intros ex Hex He Hmono.
-    eapply pure_eval_app; eauto.
-    intros c y HP ->.
-    apply pure_call_equiv.
-    apply Hmono. apply HP. }
-
-  intros ex Hex.
-  specialize (IH (P arg_head) arg_tail (EApp e ex)).
-
-  replace [ex] with ([] ++ [ex]) by reflexivity.
-  eapply pure_EApp_aSpec_induction_step.
-  { reflexivity. }
-
-  eapply pure_EApp_aSpec_mono.
-  { apply IH. }
-  intros e0; simpl.
-  intros Hpure He Hmono.
-  apply Hpure; [ | apply Hmono ].
-
-  eapply pure_eval_app; eauto.
-  intros c ? Hc ->.
-  eapply pure_call_equiv.
-  simpl in Hc |-*... rewrite args_app_bind in Hc.
-
-  eapply pure_wp_mono_throw...
-  { eapply pure_wp_mono_ret; [ by simp aSpec_aux in Hc | ].
-    intros...
-    unfold returns; eexists; split; [ reflexivity | ]...
-    done. }
-  intros ? [].
-Qed.
-
-
-
-Lemma structs_letrec (arg_τ : arg_type) `{Inhabited arg_τ}
-  (R : to_product_type arg_τ -> to_product_type arg_τ -> Prop)
-  η δ f (x : var) e (P : arg_τ -#> microvx -> Prop) sitems φ :
-  wf R ->
-  unfold_spec arg_τ η f x e (λ arg1 arg2, R (to_tuple arg1) (to_tuple arg2)) P ->
-  (∀ c, Spec c P -> struct_items ((f, c) :: η, (f, c) :: δ) sitems φ) ->
-  struct_items (η, δ) (ILetRec [RecBinding f (AnonFun x e)] :: sitems) φ.
-Proof.
-  intros Hwf Hmkspec He2.
-  unfold struct_items. simpl_eval_sitems.
-  eapply He2.
-  eapply prove_Spec_rec; eauto.
-  apply by_unfold_spec.
-  apply Hmkspec.
-Qed.
-
-(* TODO: What is this lemma doing here? *)
-Local Lemma structs_letrec_single `{Encode X} (R : X -> X -> Prop) η δ f (x : var) e
-  (P : X -> microvx -> Prop)
-  sitems φ :
-  wf R ->
-  (∀ c v',
-      Spec' c (λ v m, R v v' -> P v m) ->
-      P v' (eval ((x, #v') :: (f, c) :: η) e)) ->
-  (∀ c, Spec' c P ->
-       struct_items ((f, c) :: η, (f, c) :: δ) sitems φ) ->
-  struct_items (η, δ) (ILetRec [RecBinding f (AnonFun x e)] :: sitems) φ.
-Proof.
-  intros Hwf Hmkspec He2.
-  unfold struct_items; simpl_eval_sitems.
-  eapply He2. intros v.
-  induction v as [v IH] using (well_founded_induction Hwf); intros.
-  simpl; rewrite String.eqb_refl; simpl.
-  by eapply Hmkspec.
-Qed.
-
-
-(* [prove_Spec_recer] gives an induction principle for [Spec] by
-   well-foundedness over the argument type. *)
-
-Lemma prove_Spec_recer1 `{Encode X, Inhabited (Arg1 X)}
-  (R : X -> X -> Prop) c
-  (P : X -> microvx -> Prop) :
-  wf R ->
-  (∀ (args : X),
-      Spec c (arg_bind(λ (x : Arg1 X) m, R x args -> P x m)) ->
-    @aSpec (Arg1 X) c P args)->
-  @Spec (Arg1 X) c P.
-Proof.
-  intros Hwf HP.
-  eapply prove_Spec_rec; eassumption.
-Qed.
-
-Lemma prove_Spec_recer2 `{Encode X, Inhabited (ArgS X arg_τ)}
-  (R : ArgS X arg_τ -> ArgS X arg_τ -> Prop)
-  (P : ArgS X arg_τ -#> microvx -> Prop)
-  η f xvar af :
-  let c := VCloRec η [RecBinding f (AnonFun xvar (EAnonFun af))] f in
-  wf R ->
-  (∀ (args : ArgS X arg_τ),
-      Spec c (arg_bind(λ (x : Arg1 X) (m : microvx),
-                  ∀# (sargs : arg_τ),
-                  R (ArgCons x sargs) args ->
-                  pure m (λ c', aSpec c' (P x) sargs) ⊥)) ->
-    arg_app (@aSpec (ArgS X arg_τ) c P args.(arg_head)) args.(arg_tail))->
-  @Spec (ArgS X arg_τ) c P.
-Proof.
-  intros Hc Hwf HP.
-  eapply prove_Spec_rec; try eassumption.
-  rewrite spec_once; intros x.
-  apply forallArgs_forall; intros args.
-  intros IH.
-  rewrite spec_once in IH.
-  unfold aSpec; rewrite args_app_bind.
-  simp aSpec_aux.
-  rewrite spec_once_tele in HP.
-  specialize (HP x args).
-  unfold aSpec in HP.
-  simpl in HP; rewrite args_app_bind in HP.
-  simp aSpec_aux in HP.
-  apply HP.
-  simp Spec. intros y.
-  apply forallArgs_forall; intros sargs HR.
-  specialize (IH y). rewrite forallArgs_forall in IH.
-  specialize (IH sargs HR).
-  unfold aSpec in IH; rewrite args_app_bind in IH.
-  simp aSpec_aux in IH.
-  eapply pure_wp_mono_ret; [ apply IH | ].
-  intros c' HSpec'.
-  unfold returns; eexists; split; [ reflexivity | ].
-  rewrite args_app_bind; apply HSpec'.
-Qed.
-
-
-Lemma prove_Spec_recer `{Encode X, Encode Y, Inhabited (ArgS X (ArgS Y arg_τ))}
-  (R : ArgS X (ArgS Y arg_τ) -> ArgS X (ArgS Y arg_τ) -> Prop)
-  (P : ArgS X (ArgS Y arg_τ) -#> microvx -> Prop)
-  η f xvar yvar e :
-  let c := VCloRec η [RecBinding f
-                        (AnonFun xvar
-                           (EAnonFun
-                              (AnonFun yvar e)))] f in
-  wf R ->
-  (∀ (args : ArgS X (ArgS Y arg_τ)),
-      @Spec tele[ X; Y ] c (λ (x : X) (y : Y) (m : microvx),
-                  ∀# (sargs : arg_τ),
-                  R (ArgCons x (ArgCons y sargs)) args ->
-                  pure m (λ c', aSpec c' (P x y) sargs) ⊥) ->
-      let x := args.(arg_head) in
-      let y := args.(arg_tail).(arg_head) in
-      let args := args.(arg_tail).(arg_tail) in
-    arg_app (@aSpec (ArgS X (ArgS Y arg_τ)) c P x y) args)->
-  @Spec (ArgS X (ArgS Y arg_τ)) c P.
-Proof.
-  intros Hc Hwf HP.
-  eapply prove_Spec_rec; try eassumption.
-  rewrite spec_once; intros x.
-  rewrite spec_once; intros y.
-  apply forallArgs_forall; intros args.
-  intros IH.
-
-  unfold aSpec; rewrite args_app_bind.
-  simp aSpec_aux.
-  rewrite spec_once_tele in HP; specialize (HP x).
-  rewrite spec_once_tele in HP; specialize (HP y args).
-  simpl in HP.
-
-  unfold aSpec in HP.
-  simpl in HP; rewrite args_app_bind in HP.
-  simp aSpec_aux in HP.
-  apply HP.
-  simp Spec. intros x'.
-  simpl; rewrite String.eqb_refl; simpl; simpl_eval; apply pure_wp_ret.
-  simp Spec. intros y'.
-  apply forallArgs_forall; intros sargs HR.
-  simpl.
-
-  rewrite spec_once in IH; specialize (IH x').
-  rewrite spec_once in IH; specialize (IH y').
-  rewrite forallArgs_forall in IH; specialize (IH sargs HR).
-  unfold aSpec in IH; rewrite args_app_bind in IH.
-  simp aSpec_aux in IH.
-
-  simpl in IH; rewrite String.eqb_refl in IH; simpl in IH.
-  unfold eval in IH; rewrite seal_eq in IH; simpl in IH.
-  apply invert_pure_wp_ret in IH.
-  simp aSpec_aux in IH.
-  simpl in IH.
-  eapply pure_wp_mono_ret. apply IH.
-  intros c' HSpec'.
-  unfold returns; eexists; split; [ reflexivity | ].
-  rewrite args_app_bind; apply HSpec'.
-Qed.
+(* (* [prove_Spec_rec] gives an induction principle for [Spec] by *)
+(*    well-foundedness over the argument type. *) *)
+
+(* Lemma prove_Spec_rec {A : types} *)
+(*   (R : A -> A -> Prop) c *)
+(*   (P : A -#> microvx -> Prop) : *)
+(*   WellFounded R -> *)
+(*   (∀# (args : A), *)
+(*     (∀# sargs, R sargs args -> Spec c P) -> *)
+(*     Spec c P)-> *)
+(*   Spec c P. *)
+(* Proof. *)
+(*   intros Hwf HP. *)
+(*   apply aSpec_Spec; eauto. *)
+(*   intros args. *)
+
+(*   induction args as [args IHR] using (well_founded_induction Hwf); clear Hwf. *)
+
+(*   rewrite forallArgs_forall in HP. specialize (HP args). *)
+(*   apply HP. *)
+(*   apply forallArgs_forall; apply IHR. *)
+(* Qed. *)
